src/PermSecInstr.v
@@ -4,7 +4,8 @@ Require Export PermSec.
 
 Lemma read_secure:
   forall s pr a tb,
-    permission_secure pr s (Read a) (fun s => disk s a = Some tb) (fun s s' r => s' = blocks_upd s r tb).
+    disk s a = Some tb ->
+    permission_secure pr s (Read a) (fun s s' r => s' = blocks_upd s r tb).
 Proof.
   unfold permission_secure; intros.
   inv_exec_perm; simpl in *; cleanup.
@@ -13,8 +14,8 @@ Qed.
 
 Lemma write_secure:
   forall pr s a i tb,
-    permission_secure pr s (Write a i) (fun s => blocks s i = Some tb)
-                      (fun s s' _ => s' = disk_upd s a tb).
+    blocks s i = Some tb ->
+    permission_secure pr s (Write a i) (fun s s' _ => s' = disk_upd s a tb).
 Proof.
   unfold permission_secure; intros.
   inv_exec_perm; simpl in *; cleanup.
@@ -25,8 +26,7 @@ Qed.
 Lemma seal_secure:
   forall pr s t b,
     can_access pr t ->
-    permission_secure pr s (Seal t b) (fun _ => True)
-                      (fun s s' r => s' = blocks_upd s r (t, b)).
+    permission_secure pr s (Seal t b) (fun s s' r => s' = blocks_upd s r (t, b)).
 Proof.
   unfold permission_secure; intros.
   inv_exec_perm; simpl in *; cleanup.
@@ -36,8 +36,8 @@ Qed.
 Lemma unseal_secure:
   forall pr s i t b,
     can_access pr t ->
-    permission_secure pr s (Unseal i) (fun s => blocks s i = Some (t, b))
-                      (fun s s' r => s' = s /\ r = b).
+    blocks s i = Some (t, b) ->
+    permission_secure pr s (Unseal i) (fun s s' r => s' = s /\ r = b).
 Proof.
   unfold permission_secure; intros.
   inv_exec_perm; simpl in *; cleanup.
@@ -46,7 +46,7 @@ Qed.
 
 Lemma ret_secure:
   forall T pr s (v: T),
-    permission_secure pr s (Ret v) (fun _ => True) (fun s s' r => s' = s /\ r = v).
+    permission_secure pr s (Ret v) (fun s s' r => s' = s /\ r = v).
 Proof.
   unfold permission_secure; intros.
   inv_exec_perm; simpl in *; cleanup.
@@ -54,109 +54,72 @@ Proof.
 Qed.
 
 Lemma run_secure:
-  forall T s (p: prog T) pr pr' pre post,
-    permission_secure pr' s p pre post ->
+  forall T s (p: prog T) pr pr' post,
+    permission_secure pr' s p post ->
     permitted pr pr' ->
-    permission_secure pr s (Run pr' p) pre post.
+    permission_secure pr s (Run pr' p) post.
 Proof.
   unfold permission_secure; intros.
   inv_exec_perm; simpl in *.
-  specialize (trace_app H11); intros; cleanup.
-  specialize (H _ _ _ _ H1 H11); intuition.
+  specialize (trace_app H10); intros; cleanup.
+  specialize (H _ _ _ _ H10); intuition.
   simpl; intuition.
   eapply trace_secure_permitted; eauto.
 Qed.
 
 Lemma bind_secure:
-  forall T T' (p1: prog T) (p2: T -> prog T') t s pre post
-    (post': state -> Prop) (post2: state -> state -> T' -> Prop),
-    permission_secure t s p1 pre post ->
-    (forall s' tr tr' r,
-       pre s ->
-       exec t s tr p1 s' (Finished r) tr' ->
-       post s s' r ->
-       post' s') ->
+  forall T T' (p1: prog T) (p2: T -> prog T') pr s post
+    (post2: state -> state -> T' -> Prop),
+    permission_secure pr s p1 post ->
     (forall s' s'' tr tr' tr'' r r',
-       pre s ->
-       exec t s tr p1 s' (Finished r) tr' ->
+       exec pr s tr p1 s' (Finished r) tr' ->
        post s s' r ->
-       post' s' ->
-       exec t s' tr' (p2 r) s'' (Finished r') tr'' ->
+       exec pr s' tr' (p2 r) s'' (Finished r') tr'' ->
        post2 s' s'' r' ->
        post2 s s'' r') ->
     (forall s' tr tr' r,
-       pre s ->
-       exec t s tr p1 s' (Finished r) tr' ->
+       exec pr s tr p1 s' (Finished r) tr' ->
        post s s' r ->
-       permission_secure t s' (p2 r) post' post2 ) ->
-    permission_secure t s (Bind p1 p2) pre post2.
+       permission_secure pr s' (p2 r) post2) ->
+    permission_secure pr s (Bind p1 p2) post2.
 Proof.
   unfold permission_secure; intros.
   inv_exec_perm.
-  specialize (trace_app H4); intros; cleanup.
-  specialize (H _ _ _ _ H3 H4); cleanup.
-  specialize (trace_app H5); intros; cleanup.
-  specialize (H0 _ _ _ _ H3 H4 H6); cleanup.
-  specialize (H2 _ _ _ _ H3 H4 H6); cleanup.
-  specialize (H2 _ _ _ _ H0 H5); cleanup.
-  specialize (H1 _ _ _ _ _ _ _ H3 H4 H6 H0 H5 H7); intuition.
+  specialize (trace_app H2); intros; cleanup.
+  specialize (H _ _ _ _ H2); cleanup.
+  specialize (trace_app H3); intros; cleanup.
+  specialize (H1 _ _ _ _ H2 H4); cleanup.
+  specialize (H1 _ _ _ _ H3); cleanup.
+  intuition.
   apply trace_secure_app; auto.
+  eauto.
 Qed.
 
 
 Lemma permission_drop_secure:
-  forall s pr1 pr2 T (p: prog T) pre post,
-    permission_secure pr1 s p pre post ->
+  forall s pr1 pr2 T (p: prog T) post,
+    permission_secure pr1 s p post ->
     permitted pr2 pr1 ->
     (forall s' tr tr2 r, exec pr2 s tr p s' r (tr2++tr) ->
                       exists tr1, exec pr1 s tr p s' r (tr1++tr) /\ trace_match pr1 pr2 tr1 tr2) ->
-    permission_secure pr2 s p pre post.
+    permission_secure pr2 s p post.
 Proof.
   unfold permission_secure; intros.
-  specialize (H1 _ _ _ _ H3); cleanup.
-  specialize (H _ _ _ _ H2 H1); intuition.
+  specialize (H1 _ _ _ _ H2); cleanup.
+  specialize (H _ _ _ _ H1); intuition.
   eapply trace_secure_match; eauto.
 Qed.
 
-
-Theorem pre_impl_secure:
-  forall T s (p: prog T) pr (pre pre': PermProg.state -> Prop) post,
-    permission_secure pr s p pre' post ->
-    (pre s -> pre' s) ->
-    permission_secure pr s p pre post.
-Proof.
-  unfold permission_secure; intros.
-  specialize (H0 H1); eauto.
-Qed.
-
-Theorem post_impl_secure:
-  forall T s (p: prog T) pr (pre: PermProg.state -> Prop)
-    (post post': PermProg.state -> PermProg.state -> T -> Prop),
-    permission_secure pr s p pre post ->
-    (forall s' tr tr' r,
-       pre s ->
-       exec pr s tr p s' (Finished r) tr' ->
-       post s s' r ->
-       post' s s' r) ->
-    permission_secure pr s p pre post'.
-Proof.
-  unfold permission_secure; intros.
-  specialize (H _ _ _ _ H1 H2); cleanup; eauto.
-Qed. 
-
 Theorem impl_secure:
-  forall T s (p: prog T) pr (pre pre': PermProg.state -> Prop)
+  forall T s (p: prog T) pr
     (post post': PermProg.state -> PermProg.state -> T -> Prop),
-    permission_secure pr s p pre' post ->
+    permission_secure pr s p post ->
     (forall s' tr tr' r,
-       pre' s ->
        exec pr s tr p s' (Finished r) tr' ->
        post s s' r ->
        post' s s' r) ->
-    (pre s -> pre' s) ->
-    permission_secure pr s p pre post'.
+    permission_secure pr s p post'.
 Proof.
-  intros;
-  eapply pre_impl_secure; eauto.
-  eapply post_impl_secure; eauto.
+  unfold permission_secure; intros.
+  specialize (H _ _ _ _ H1); cleanup; eauto.
 Qed. 
